theories/ordinals/Ackermann/LNT.v
@@ -17,13 +17,13 @@ Definition Terms := Terms LNT.
 Definition SysPrf := SysPrf LNT.
 
 Definition Plus (x y : Term) : Term :=
-  @apply LNT Plus (Tcons 1 x (Tcons 0 y (Tnil))).
+  @apply LNT Plus (Tcons x (Tcons y (Tnil))).
 
 Definition Times (x y : Term) : Term :=
-  @apply LNT Times (Tcons 1 x (Tcons 0 y (Tnil))).
+  @apply LNT Times (Tcons x (Tcons y (Tnil))).
 
 Definition Succ (x : Term) : Term :=
-  @apply LNT Succ (Tcons 0 x (Tnil)).
+  @apply LNT Succ (Tcons x (Tnil)).
 
 Definition Zero : Term := @apply LNT Zero (Tnil).
 
@@ -243,8 +243,8 @@ Proof.
   intros H H0; unfold Plus.
   apply (equalFunction LNT).
   simpl in |- *.
-  destruct (consTerms LNT 1 (Tcons 1 a (Tcons 0 c (Tnil))))as [(a0,b0) p].
-  simpl; destruct (consTerms LNT 1 (Tcons 1 b (Tcons 0 d (Tnil)))) 
+  destruct (consTerms LNT 1 (Tcons a (Tcons c (Tnil))))as [(a0,b0) p].
+  simpl; destruct (consTerms LNT 1 (Tcons b (Tcons d (Tnil)))) 
     as [(a1,b1) p0]. 
   simpl in |- *.
   destruct (consTerms LNT 0 b0) as [(a2,b2) p1]. 
@@ -274,9 +274,9 @@ Lemma eqTimes  (T : System) (a b c d : Term):
 Proof.
   intros H H0; unfold Times in |- *.
   apply (equalFunction LNT); simpl in |- *.
-  destruct (consTerms LNT 1 (Tcons 1 a (Tcons 0 c (Tnil))))as [(a0,b0) p].
+  destruct (consTerms LNT 1 (Tcons a (Tcons c (Tnil))))as [(a0,b0) p].
   simpl in |- *.
-  destruct (consTerms LNT 1 (Tcons 1 b (Tcons 0 d (Tnil)))) as [(a1,b1) p0].
+  destruct (consTerms LNT 1 (Tcons b (Tcons d (Tnil)))) as [(a1,b1) p0].
   simpl; destruct (consTerms LNT 0 b0) as [(a2,b2) p1].
   simpl ; destruct (consTerms LNT 0 b1) as [(a3,b3) p2].
   simpl in |- *; repeat split.
@@ -302,9 +302,9 @@ Lemma eqSucc (T : System) (a b : Term):
 Proof.
   intros H; unfold Succ in |- *; apply (equalFunction LNT).
   simpl in |- *.
-  destruct (consTerms LNT 0 (Tcons 0 a (Tnil))) as [(a0,b0) p].
+  destruct (consTerms LNT 0 (Tcons a (Tnil))) as [(a0,b0) p].
   simpl in |- *;
-destruct (consTerms LNT 0 (Tcons 0 b (Tnil))) as [(a1,b1) p0].
+destruct (consTerms LNT 0 (Tcons b (Tnil))) as [(a1,b1) p0].
   simpl in |- *; repeat split.
   - simpl in p.
     inversion p.
