theories/goedel/PRrepresentable.v
@@ -181,7 +181,7 @@ Proof.
                         **** (* fold (var 4) in |- *. *)
                              replace 
                                (@apply LNN Languages.Succ 
-                                  (Tcons 0 (natToTerm a)
+                                  (Tcons (natToTerm a)
                                      (Tnil)))
                                with (natToTerm (S a)); 
                                [| reflexivity ].
@@ -253,9 +253,8 @@ Proof.
                                  * apply sysWeaken.
                                    replace
                                      (@apply LNN Languages.Succ
-                                        (Tcons 0
-                                           (@apply LNN Languages.Succ
-                                              (Tcons 0
+                                        (Tcons (@apply LNN Languages.Succ
+                                              (Tcons 
                                                  (@apply LNN Languages.Zero
                                                     (Tnil))
                                                  (Tnil)))
@@ -409,18 +408,17 @@ Proof.
                                                   with
                                                     (fol.equal 
                                                        (@apply LNN Languages.Plus
-                                                          (Tcons 1 (natToTerm n)
-                                                             (Tcons 0
-                                                                (@apply LNN Languages.Times
-                                                                   (Tcons 1 (var  5)
-                                                                      (Tcons 0
+                                                          (Tcons (natToTerm n)
+                                                             (Tcons                                                                 (@apply LNN Languages.Times
+                                                                   (Tcons (var  5)
+                                                                      (Tcons 
                                                                          (@apply LNN Languages.Succ
-                                                                            (Tcons 0
+                                                                            (Tcons 
                                                                                (@apply LNN Languages.Times
-                                                                                  (Tcons 1 (natToTerm (cPairPi1 a))
-                                                                                     (Tcons 0
+                                                                                  (Tcons  (natToTerm (cPairPi1 a))
+                                                                                     (Tcons 
                                                                                         (@apply LNN Languages.Succ
-                                                                                           (Tcons 0 
+                                                                                           (Tcons  
                                                                                               (natToTerm a0) 
                                                                                               (Tnil))) 
                                                                                         (Tnil)))) 
@@ -449,18 +447,18 @@ Proof.
                                                           ** apply eqSym. apply natPlus.
                                                           ** replace
                                                               (@apply LNN Languages.Plus
-                                                                 (Tcons 1 (natToTerm n)
-                                                                    (Tcons 0
+                                                                 (Tcons  (natToTerm n)
+                                                                    (Tcons 
                                                                        (@apply LNN Languages.Times
-                                                                          (Tcons 1 (natToTerm n0)
-                                                                             (Tcons 0
+                                                                          (Tcons  (natToTerm n0)
+                                                                             (Tcons 
                                                                                 (@apply LNN Languages.Succ
-                                                                                   (Tcons 0
+                                                                                   (Tcons 
                                                                                       (@apply LNN Languages.Times
-                                                                                         (Tcons 1 (natToTerm (cPairPi1 a))
-                                                                                            (Tcons 0
+                                                                                         (Tcons  (natToTerm (cPairPi1 a))
+                                                                                            (Tcons 
                                                                                                (@apply LNN Languages.Succ
-                                                                                                  (Tcons 0 (natToTerm a0) (Tnil)))
+                                                                                                  (Tcons (natToTerm a0) (Tnil)))
                                                                                                (Tnil )))) (Tnil ))) 
                                                                                 (Tnil )))) (Tnil )))) with
                                                               (Plus (natToTerm n)
@@ -498,7 +496,7 @@ Proof.
         induction x as (a1, b). simpl in |- *. simpl in H1. destruct H1 as (H1, H2).
         apply existI with (natToTerm (cPairPi1 a)). rewrite (subFormulaAnd LNN). apply andI.
         ++ apply sysWeaken. rewrite H0. simpl in |- *. rewrite subTermNil.
-           -- replace (@apply LNN Languages.Succ (Tcons 0 (natToTerm a) (Tnil ))) with (natToTerm (S a)) by reflexivity.
+           -- replace (@apply LNN Languages.Succ (Tcons (natToTerm a) (Tnil ))) with (natToTerm (S a)) by reflexivity.
               apply natLT. apply Nat.lt_succ_r. apply Nat.le_trans with (cPair (cPairPi1 a) (cPairPi2 a)).
               apply cPairLe1. rewrite cPairProjections. apply le_n.
            -- apply closedNatToTerm.
@@ -506,7 +504,7 @@ Proof.
            -- apply existI with (natToTerm (cPairPi2 a)). repeat rewrite (subFormulaAnd LNN). apply andI.
               ** apply sysWeaken. repeat rewrite H0. simpl in |- *.
                  repeat rewrite (subTermNil LNN (natToTerm a)).
-                 +++ replace (@apply LNN Languages.Succ (Tcons 0 (natToTerm a) (Tnil ))) with (natToTerm (S a)) by reflexivity.
+                 +++ replace (@apply LNN Languages.Succ (Tcons (natToTerm a) (Tnil ))) with (natToTerm (S a)) by reflexivity.
                      apply natLT. apply Nat.lt_succ_r. apply Nat.le_trans with (cPair (cPairPi1 a) (cPairPi2 a)).
                      --- apply cPairLe2.
                      --- rewrite cPairProjections. apply le_n.
@@ -522,39 +520,39 @@ Proof.
                      replace
                       (fol.equal 
                          (@apply LNN Languages.Plus
-                            (Tcons 1
+                            (Tcons
                                (@apply LNN Languages.Times
-                                  (Tcons 1
+                                  (Tcons
                                      (@apply LNN Languages.Plus
-                                        (Tcons 1 (natToTerm (cPairPi1 a))
-                                           (Tcons 0 (natToTerm (cPairPi2 a)) (Tnil ))))
-                                     (Tcons 0
+                                        (Tcons (natToTerm (cPairPi1 a))
+                                           (Tcons (natToTerm (cPairPi2 a)) (Tnil ))))
+                                     (Tcons
                                         (@apply LNN Languages.Succ
-                                           (Tcons 0
+                                           (Tcons
                                               (@apply LNN Languages.Plus
-                                                 (Tcons 1 (natToTerm (cPairPi1 a))
-                                                    (Tcons 0 (natToTerm (cPairPi2 a))
+                                                 (Tcons (natToTerm (cPairPi1 a))
+                                                    (Tcons (natToTerm (cPairPi2 a))
                                                        (Tnil )))) (Tnil )))
                                         (Tnil))))
-                               (Tcons 0
+                               (Tcons
                                   (@apply LNN Languages.Times
-                                     (Tcons 1
+                                     (Tcons
                                         (@apply LNN Languages.Succ
-                                           (Tcons 0
+                                           (Tcons
                                               (@apply LNN Languages.Succ
-                                                 (Tcons 0
+                                                 (Tcons
                                                     (@apply LNN Languages.Zero (Tnil ))
                                                     (Tnil ))) (Tnil )))
-                                        (Tcons 0 (natToTerm (cPairPi1 a)) (Tnil ))))
+                                        (Tcons (natToTerm (cPairPi1 a)) (Tnil ))))
                                   (Tnil ))))
                          (@apply LNN Languages.Times
-                            (Tcons 1
+                            (Tcons
                                (@apply LNN Languages.Succ
-                                  (Tcons 0
+                                  (Tcons
                                      (@apply LNN Languages.Succ
-                                        (Tcons 0 (@apply LNN Languages.Zero (Tnil ))
+                                        (Tcons (@apply LNN Languages.Zero (Tnil ))
                                            (Tnil ))) (Tnil )))
-                               (Tcons 0 (natToTerm a) (Tnil ))))) with
+                               (Tcons (natToTerm a) (Tnil ))))) with
                       (equal
                          (Plus
                             (Times (Plus (natToTerm (cPairPi1 a)) (natToTerm (cPairPi2 a)))
@@ -670,22 +668,22 @@ Proof.
                              repeat
                               (rewrite (subTermNil LNN (natToTerm a1)); [| apply closedNatToTerm ]).
                              apply andI.
-                             ++++ replace (@apply LNN Languages.Succ (Tcons 0 (natToTerm (cPairPi2 a)) (Tnil ))) with (natToTerm (S (cPairPi2 a))) by reflexivity.
+                             ++++ replace (@apply LNN Languages.Succ (Tcons (natToTerm (cPairPi2 a)) (Tnil ))) with (natToTerm (S (cPairPi2 a))) by reflexivity.
                                   apply natLT. unfold coPrimeBeta in *. lia.
                              ++++ replace
                                    (@apply LNN Languages.Plus
-                                      (Tcons 1 (natToTerm b)
-                                         (Tcons 0
+                                      (Tcons (natToTerm b)
+                                         (Tcons
                                             (@apply LNN Languages.Times
-                                               (Tcons 1 (natToTerm a1)
-                                                  (Tcons 0
+                                               (Tcons (natToTerm a1)
+                                                  (Tcons
                                                      (@apply LNN Languages.Succ
-                                                        (Tcons 0
+                                                        (Tcons
                                                            (@apply LNN Languages.Times
-                                                              (Tcons 1 (natToTerm (cPairPi1 a))
-                                                                 (Tcons 0
+                                                              (Tcons (natToTerm (cPairPi1 a))
+                                                                 (Tcons
                                                                     (@apply LNN Languages.Succ
-                                                                       (Tcons 0 (natToTerm a0) (Tnil )))
+                                                                       (Tcons (natToTerm a0) (Tnil )))
                                                                     (Tnil )))) (Tnil ))) 
                                                      (Tnil )))) (Tnil )))) with
                                    (Plus (natToTerm b)
