theories/ordinals/Ackermann/PAtheory.v
@@ -159,8 +159,8 @@ Proof.
                      fold
                        (Succ
                           (@apply LNT Languages.Plus
-                             (Tcons 1 (var 1) 
-                                (Tcons 0 Zero (Tnil))))) 
+                             (Tcons (var 1) 
+                                (Tcons Zero (Tnil))))) 
                        in |- *.
                      apply eqSucc.
                      apply pa3 with (a := var 1).
@@ -177,8 +177,8 @@ Proof.
                      fold
                        (Succ
                           (@apply LNT Languages.Plus
-                             (Tcons 1 (var 1)
-                                (Tcons 0 (Succ (var 0)) (Tnil)))))
+                             (Tcons (var 1)
+                                (Tcons (Succ (var 0)) (Tnil)))))
                        in |- *.
                      apply eqSucc.
                      apply eqTrans with (Succ (Plus (var 1) (var 0))).
