theories/ordinals/Ackermann/fol.v
@@ -726,4 +726,4 @@ Arguments atomic {L} _ _.
 Arguments apply {L} _ _.
 Arguments ifThenElseH {L} _ _ _.
 Arguments Tnil {L}.
-Arguments Tcons {L} _ _ _.
+Arguments Tcons {L} {n} _ _.
